progress on byte disjointness

HOL/panScript.sml
@@ -109,9 +109,9 @@ Theorem valid_value_simp[simp] = is_valid_value_def;
 Theorem shape_of_simp[simp] = shape_of_def;
 Theorem h_prog_skip[simp] = cj 1 h_prog_def;
 
-val assign_tac = gvs[Once itree_mrec_alt, Once h_prog_def,
+val assign_tac = gvs[Once itree_mrec_def, Once h_prog_def,
                      h_prog_rule_assign_def, eval_def];
-val strb_tac = rw[Once itree_mrec_alt, Once h_prog_def, h_prog_rule_store_byte_def];
+val strb_tac = rw[Once itree_mrec_def, Once h_prog_def, h_prog_rule_store_byte_def];
 Globals.max_print_depth := 25;
 
 (*/ word nonsense
@@ -172,50 +172,143 @@ End
   writes within boundaries (not necessarily current) preserve wf
 
   making new regions requires quadratic obligations for disjointness
-
-  maybe look into fun2set in set_sepScript
  *)
 
-(* Definition writes_disjoint_def: *)
-(*   write_disjoint (s1,l1) (s2,l2) *)
-(*   = ((s1 + n2w(LENGTH l1) < s2) ∨ (s2 + n2w(LENGTH l2) < s1)) *)
-(* End *)
+Type write[pp] = “:(num # word8 list)”;
+Type range[pp] = “:(num # num)”;
+Definition range_disjoint_def:
+  range_disjoint ((s1,l1) : range) ((s2,l2) : range)
+  = ((s1 + l1 < s2) ∨ (s2 + l2 < s1))
+End
 
-(* Inductive wordf: *)
-(*   (wordf []) ∧ *)
-(*   (EVERY (write_disjoint a) as ∧ wordf as ⇒ wordf (a::as)) *)
-(* End *)
+Definition writes_disjoint_def:
+  write_disjoint ((s1,l1) : write) ((s2,l2) : write)
+  = range_disjoint (s1, LENGTH l1) (s2, LENGTH l2)
+End
 
-(* Definition bwrites_def: *)
-(*   bwrites [] s = s.memory ∧ *)
-(*   bwrites ((off,l)::as) s *)
-(*   = write_bytearray (s.base_addr + off) l (bwrites as s) s.memaddrs s.be *)
-(* End *)
+Theorem write_bytearray_preserve_words:
+  mem_has_word oldmem w ⇒
+  mem_has_word (write_bytearray loc l oldmem s.memaddrs s.be) w
+Proof
+  simp[mem_has_word_def] >>
+  strip_tac >>
+  qid_spec_tac ‘loc’ >> Induct_on ‘l’ >>
+  rw[write_bytearray_def] >>
+  fs[mem_store_byte_def] >>
+  Cases_on ‘write_bytearray (loc+1w) l oldmem s.memaddrs s.be (byte_align loc)’ >>
+  rw[] >>
+  rw[combinTheory.APPLY_UPDATE_THM]
+QED
 
-(* Theorem join_bwrites: *)
-(*   write_bytearray (s.base_addr + off) bs (bwrites [] s) s.memaddrs s.be *)
-(* Proof *)
-(* QED *)
+Theorem disjoint_write_byte:
+  (∀a. a ∈ s.memaddrs) ∧
+  (∀a. a < n2w q + n2w (LENGTH r) ⇒ mem_has_word s.memory a)
+  ∧
+  range_disjoint (start, len) (q, LENGTH r) ∧
+  start ≤ pos ∧ pos < len + start
+  ⇒
+  mem_load_byte
+  (write_bytearray (n2w q) r s.memory s.memaddrs s.be)
+  s.memaddrs s.be (n2w pos)
+  = mem_load_byte s.memory s.memaddrs s.be (n2w pos)
+Proof
+  rw[range_disjoint_def] >-
+   (‘pos < q’ by rw[] >>
+    qpat_x_assum ‘pos < _ + _’ kall_tac >>
+    qpat_x_assum ‘_ ≤ _’ kall_tac >>
+    qpat_x_assum ‘_ + _ < _’ kall_tac >>
+    pop_assum mp_tac >> pop_assum mp_tac >>
+    qid_spec_tac ‘q’ >>
+    Induct_on ‘r’ >>
+    rw[write_bytearray_def] >>
+    rw[mem_store_byte_def] >>
+    ‘mem_has_word
+     (write_bytearray (n2w q + 1w) r s.memory s.memaddrs s.be)
+     (n2w q)’ by cheat >>
+    fs[mem_has_word_def] >>
+    simp[mem_load_byte_def, SimpL “$=”] >>
+    ‘byte_align (n2w q) ≠ byte_align (n2w pos) : word32’ by cheat >>
+    simp[cj 2 combinTheory.UPDATE_APPLY] >>
+    last_x_assum $ qspec_then ‘q + 1’ strip_assume_tac >> gvs[] >>
+    ‘n2w q + 1w = n2w (q + 1) : word32’
+      by metis_tac[arithmeticTheory.SUC_ONE_ADD, arithmeticTheory.ADD_COMM,
+                   wordsTheory.n2w_SUC] >>
+    ‘n2w (LENGTH r) + n2w (q + 1) = n2w q + n2w (SUC (LENGTH r)) : word32’
+      by metis_tac[wordsTheory.WORD_ADD_ASSOC, wordsTheory.WORD_ADD_COMM,
+                   wordsTheory.n2w_SUC] >>
+    gvs[mem_load_byte_def]) >-
+   (cheat
+   )
+QED
 
-(* Theorem test: *)
-(*   (write_bytearray *)
-(*   (s.base_addr + (3w : word32)) [x] *)
-(*   (write_bytearray (s.base_addr + 1w) [c] s.memory *)
-(*                    s.memaddrs s.be) s.memaddrs s.be) *)
-(*   = *)
-(*   bwrites [(3w : word32,[x]);(1w : word32,[c])] s *)
-(* Proof *)
-(*   rw[bwrites_def] *)
-(* QED *)
+Inductive wordf:
+  (wordf []) ∧
+  (EVERY (write_disjoint a) as ∧ wordf as ⇒ wordf (a::as))
+End
 
-(* Theorem test2: *)
-(*   wordf [(3w : word32,[x]);(1w : word32,[c])] *)
-(* Proof *)
-(*   rw[Once wordf_cases] >- *)
-(*    (rw[writes_disjoint_def]) >> *)
-(*   rw[Once wordf_cases] >> *)
-(*   rw[Once wordf_cases] *)
-(* QED *)
+Theorem wordf_test:
+  wordf [(3,[x]);(1,[c])]
+Proof
+  rw[Once wordf_cases] >-
+   (rw[writes_disjoint_def]) >>
+  rw[Once wordf_cases] >>
+  rw[Once wordf_cases]
+QED
+
+Definition bwrites_def:
+  bwrites ([] : write list) s = s.memory ∧
+  bwrites ((off,l)::as) s
+  = write_bytearray (s.base_addr + (n2w off)) l (bwrites as s) s.memaddrs s.be
+End
+
+Theorem bwrites_test:
+  (write_bytearray
+  (s.base_addr + (3w : word32)) [x]
+  (write_bytearray (s.base_addr + 1w) [c] s.memory
+                   s.memaddrs s.be) s.memaddrs s.be)
+  =
+  bwrites [(3,[x]);(1,[c])] s
+Proof
+  rw[bwrites_def]
+QED
+
+Definition find_range:
+  find_range (off,len) writes
+  = FIND (λ(start : num, l : word8 list).
+            start ≤ off ∧ off + len ≤ start + (LENGTH l)) writes
+End
+
+Theorem find_test:
+  ∃v. find_range (1,1) [(3,[x]);(1,[c])] = SOME v
+Proof
+  rw[find_range, FIND_thm]
+QED
+
+Theorem join_bwrites:
+  write_bytearray (s.base_addr + off) bs (bwrites [] s) s.memaddrs s.be
+Proof
+QED
+
+Definition range_at:
+  range_at (start,len) pos (b : word8) (s : ('a, 'b) bstate)
+  = (start ≤ pos ∧ (pos < start + len) ∧
+     mem_load_byte s.memory s.memaddrs s.be (n2w pos) = SOME b)
+End
+
+Definition ranged_pred:
+  ranged_pred P start len =
+  (∀(w : write) (s : ('a, 'b) bstate).
+     P s ∧ range_disjoint (start, len) (FST w, LENGTH (SND w))
+     ⇒ P (s with memory := (bwrites [w] s)))
+End
+
+Theorem at_ranged:
+  ranged_pred (range_at (start, len) pos b) start len
+Proof
+  rw[ranged_pred, range_at] >>
+  Cases_on ‘w’ >> fs[bwrites_def] >>
+  rw[disjoint_write_byte]
+QED
 
 (*
   old byte theorems
@@ -293,20 +386,6 @@ Proof
   Cases_on ‘smem (byte_align other)’ >> gvs[] >>
   Cases_on ‘byte_align addr = byte_align other’ >> gvs[] >>
   rw[combinTheory.UPDATE_APPLY]
-QED
-
-Theorem write_bytearray_preserve_words:
-  mem_has_word oldmem w ⇒
-  mem_has_word (write_bytearray loc l oldmem s.memaddrs s.be) w
-Proof
-  simp[mem_has_word_def] >>
-  strip_tac >>
-  qid_spec_tac ‘loc’ >> Induct_on ‘l’ >>
-  rw[write_bytearray_def] >>
-  fs[mem_store_byte_def] >>
-  Cases_on ‘write_bytearray (loc+1w) l oldmem s.memaddrs s.be (byte_align loc)’ >>
-  rw[] >>
-  rw[combinTheory.APPLY_UPDATE_THM]
 QED
 
 Theorem baseaddr_ref[simp]:
